Too much procrastination

thy/Iptables_Semantics/Alternative_Semantics.thy
@@ -2,9 +2,11 @@ theory Alternative_Semantics
 imports Semantics
 begin
   
+context begin
+  
 (* the first thing (I think) we have to do is alter the Seq rule / merge it with NoMatch.
  Its properties make it hard to work with\<dots> *)
-inductive iptables_bigstep_ns :: "'a ruleset \<Rightarrow> ('a, 'p) matcher \<Rightarrow> 'p \<Rightarrow> 'a rule list \<Rightarrow> state \<Rightarrow> state \<Rightarrow> bool"
+private inductive iptables_bigstep_ns :: "'a ruleset \<Rightarrow> ('a, 'p) matcher \<Rightarrow> 'p \<Rightarrow> 'a rule list \<Rightarrow> state \<Rightarrow> state \<Rightarrow> bool"
   ("_,_,_\<turnstile> \<langle>_, _\<rangle> \<Rightarrow>\<^sub>s _"  [60,60,60,20,98,98] 89)
   for \<Gamma> and \<gamma> and p where
 skip:    "\<Gamma>,\<gamma>,p\<turnstile> \<langle>[], t\<rangle> \<Rightarrow>\<^sub>s t" |
@@ -24,7 +26,7 @@ call_no_result:  "\<lbrakk> matches \<gamma> m p; \<Gamma> chain = Some rs; \<Ga
                     \<Gamma>,\<gamma>,p\<turnstile> \<langle>rrs, Undecided\<rangle> \<Rightarrow>\<^sub>s t \<rbrakk> \<Longrightarrow>
                \<Gamma>,\<gamma>,p\<turnstile> \<langle>Rule m (Call chain) # rrs, Undecided\<rangle> \<Rightarrow>\<^sub>s t"
 
-lemma a: "\<Gamma>,\<gamma>,p\<turnstile> \<langle>rs, s\<rangle> \<Rightarrow>\<^sub>s t \<Longrightarrow> \<Gamma>,\<gamma>,p\<turnstile> \<langle>rs, s\<rangle> \<Rightarrow> t"
+private lemma a: "\<Gamma>,\<gamma>,p\<turnstile> \<langle>rs, s\<rangle> \<Rightarrow>\<^sub>s t \<Longrightarrow> \<Gamma>,\<gamma>,p\<turnstile> \<langle>rs, s\<rangle> \<Rightarrow> t"
   apply(induction rule: iptables_bigstep_ns.induct; (simp add: iptables_bigstep.intros;fail)?)
   apply (meson iptables_bigstep.decision iptables_bigstep.accept seq_cons)
   apply (meson iptables_bigstep.decision iptables_bigstep.drop seq_cons)
@@ -37,9 +39,9 @@ lemma a: "\<Gamma>,\<gamma>,p\<turnstile> \<langle>rs, s\<rangle> \<Rightarrow>\
   apply (meson iptables_bigstep.call_result seq'_cons)
   done
 
-lemma empty_rs_stateD: assumes "\<Gamma>,\<gamma>,p\<turnstile> \<langle>[], s\<rangle> \<Rightarrow>\<^sub>s t" shows "t = s"
+private lemma empty_rs_stateD: assumes "\<Gamma>,\<gamma>,p\<turnstile> \<langle>[], s\<rangle> \<Rightarrow>\<^sub>s t" shows "t = s"
   using assms by(cases rule: iptables_bigstep_ns.cases)
-lemma decided: "\<lbrakk>\<Gamma>,\<gamma>,p\<turnstile> \<langle>rs\<^sub>1, Undecided\<rangle> \<Rightarrow>\<^sub>s Decision X\<rbrakk> \<Longrightarrow> \<Gamma>,\<gamma>,p\<turnstile> \<langle>rs\<^sub>1@rs\<^sub>2, Undecided\<rangle> \<Rightarrow>\<^sub>s Decision X"
+private lemma decided: "\<lbrakk>\<Gamma>,\<gamma>,p\<turnstile> \<langle>rs\<^sub>1, Undecided\<rangle> \<Rightarrow>\<^sub>s Decision X\<rbrakk> \<Longrightarrow> \<Gamma>,\<gamma>,p\<turnstile> \<langle>rs\<^sub>1@rs\<^sub>2, Undecided\<rangle> \<Rightarrow>\<^sub>s Decision X"
 proof(induction rs\<^sub>1)
   case Nil
   then show ?case by (fast dest: empty_rs_stateD)
@@ -49,10 +51,10 @@ next
     by(cases rule: iptables_bigstep_ns.cases; simp add: Cons.IH iptables_bigstep_ns.intros)
 qed
   
-lemma decided_determ: "\<lbrakk>\<Gamma>,\<gamma>,p\<turnstile> \<langle>rs\<^sub>1, s\<rangle> \<Rightarrow>\<^sub>s t; s = Decision X\<rbrakk> \<Longrightarrow> t = Decision X"
+private lemma decided_determ: "\<lbrakk>\<Gamma>,\<gamma>,p\<turnstile> \<langle>rs\<^sub>1, s\<rangle> \<Rightarrow>\<^sub>s t; s = Decision X\<rbrakk> \<Longrightarrow> t = Decision X"
   by(induction rule: iptables_bigstep_ns.induct; (simp add: iptables_bigstep_ns.intros;fail)?)
 
-lemma seq_ns:
+private lemma seq_ns:
   "\<lbrakk>\<Gamma>,\<gamma>,p\<turnstile> \<langle>rs\<^sub>1, Undecided\<rangle> \<Rightarrow>\<^sub>s t; \<Gamma>,\<gamma>,p\<turnstile> \<langle>rs\<^sub>2, t\<rangle> \<Rightarrow>\<^sub>s t'\<rbrakk> \<Longrightarrow> \<Gamma>,\<gamma>,p\<turnstile> \<langle>rs\<^sub>1@rs\<^sub>2, Undecided\<rangle> \<Rightarrow>\<^sub>s t'"
 proof (cases t, goal_cases)
   case 1
@@ -69,13 +71,13 @@ next
   from 2(1) show ?case by (simp add: "2"(3) \<open>t' = Decision X\<close> decided)
 qed
       
-lemma b: "\<Gamma>,\<gamma>,p\<turnstile> \<langle>rs, s\<rangle> \<Rightarrow> t \<Longrightarrow> s = Undecided \<Longrightarrow> \<Gamma>,\<gamma>,p\<turnstile> \<langle>rs, s\<rangle> \<Rightarrow>\<^sub>s t"
+private lemma b: "\<Gamma>,\<gamma>,p\<turnstile> \<langle>rs, s\<rangle> \<Rightarrow> t \<Longrightarrow> s = Undecided \<Longrightarrow> \<Gamma>,\<gamma>,p\<turnstile> \<langle>rs, s\<rangle> \<Rightarrow>\<^sub>s t"
   apply(induction rule: iptables_bigstep.induct; (simp add: iptables_bigstep_ns.intros;fail)?)
    apply (metis decided decision seq_ns seq_progress skipD state.exhaust)
   apply(metis call_no_result iptables_bigstep_ns.call_result iptables_bigstep_ns.skip state.exhaust)
   done
     
-inductive iptables_bigstep_nz :: "'a ruleset \<Rightarrow> ('a, 'p) matcher \<Rightarrow> 'p \<Rightarrow> 'a rule list \<Rightarrow> state \<Rightarrow> bool"
+private inductive iptables_bigstep_nz :: "'a ruleset \<Rightarrow> ('a, 'p) matcher \<Rightarrow> 'p \<Rightarrow> 'a rule list \<Rightarrow> state \<Rightarrow> bool"
   ("_,_,_\<turnstile> _ \<Rightarrow>\<^sub>z _"  [60,60,60,20,98] 89)
   for \<Gamma> and \<gamma> and p where
 skip:    "\<Gamma>,\<gamma>,p \<turnstile> []  \<Rightarrow>\<^sub>z Undecided" |
@@ -94,10 +96,10 @@ call_no_result:  "\<lbrakk> matches \<gamma> m p; \<Gamma> chain = Some rs; \<Ga
                     \<Gamma>,\<gamma>,p\<turnstile> rrs \<Rightarrow>\<^sub>z t \<rbrakk> \<Longrightarrow>
                \<Gamma>,\<gamma>,p\<turnstile> Rule m (Call chain) # rrs \<Rightarrow>\<^sub>z t"
 
-lemma c: "\<Gamma>,\<gamma>,p\<turnstile> rs \<Rightarrow>\<^sub>z t \<Longrightarrow> \<Gamma>,\<gamma>,p\<turnstile> \<langle>rs, Undecided\<rangle> \<Rightarrow>\<^sub>s t"
+private lemma c: "\<Gamma>,\<gamma>,p\<turnstile> rs \<Rightarrow>\<^sub>z t \<Longrightarrow> \<Gamma>,\<gamma>,p\<turnstile> \<langle>rs, Undecided\<rangle> \<Rightarrow>\<^sub>s t"
   by(induction rule: iptables_bigstep_nz.induct; simp add: iptables_bigstep_ns.intros)
     
-lemma d: "\<Gamma>,\<gamma>,p\<turnstile> \<langle>rs, s\<rangle> \<Rightarrow>\<^sub>s t \<Longrightarrow> s = Undecided \<Longrightarrow> \<Gamma>,\<gamma>,p\<turnstile> rs \<Rightarrow>\<^sub>z t"
+private lemma d: "\<Gamma>,\<gamma>,p\<turnstile> \<langle>rs, s\<rangle> \<Rightarrow>\<^sub>s t \<Longrightarrow> s = Undecided \<Longrightarrow> \<Gamma>,\<gamma>,p\<turnstile> rs \<Rightarrow>\<^sub>z t"
   by(induction rule: iptables_bigstep_ns.induct; simp add: iptables_bigstep_nz.intros)
     
 inductive iptables_bigstep_r :: "'a ruleset \<Rightarrow> ('a, 'p) matcher \<Rightarrow> 'p \<Rightarrow> 'a rule list \<Rightarrow> state \<Rightarrow> bool"
@@ -113,7 +115,7 @@ empty:   "\<Gamma>,\<gamma>,p\<turnstile> rs \<Rightarrow>\<^sub>r t \<Longright
 nms:     "\<not> matches \<gamma> m p \<Longrightarrow> \<Gamma>,\<gamma>,p\<turnstile> rs \<Rightarrow>\<^sub>r t \<Longrightarrow> \<Gamma>,\<gamma>,p\<turnstile> Rule m a # rs \<Rightarrow>\<^sub>r t" |
 call_result:  "\<lbrakk> matches \<gamma> m p; \<Gamma> chain = Some rs; \<Gamma>,\<gamma>,p\<turnstile> rs \<Rightarrow>\<^sub>r Decision X \<rbrakk> \<Longrightarrow>
                \<Gamma>,\<gamma>,p\<turnstile> Rule m (Call chain) # rrs \<Rightarrow>\<^sub>r Decision X" |
-call_no_result:  "\<lbrakk> matches \<gamma> m p; \<Gamma> chain = Some rs; \<Gamma>,\<gamma>,p\<turnstile> rs \<Rightarrow>\<^sub>r Undecided;
+call_no_result:  "\<lbrakk> \<Gamma> chain = Some rs; \<Gamma>,\<gamma>,p\<turnstile> rs \<Rightarrow>\<^sub>r Undecided;
                     \<Gamma>,\<gamma>,p\<turnstile> rrs \<Rightarrow>\<^sub>r t \<rbrakk> \<Longrightarrow>
                \<Gamma>,\<gamma>,p\<turnstile> Rule m (Call chain) # rrs \<Rightarrow>\<^sub>r t"
 
@@ -121,7 +123,7 @@ lemma "\<Gamma>,\<gamma>,p\<turnstile> rs \<Rightarrow>\<^sub>r t \<Longrightarr
   apply(induction rule: iptables_bigstep_r.induct; (simp add: iptables_bigstep_nz.intros)?)
   oops
 
-lemma returning:  "\<lbrakk>\<Gamma>,\<gamma>,p\<turnstile> rs\<^sub>1 \<Rightarrow>\<^sub>r Undecided; matches \<gamma> m' p\<rbrakk>
+private lemma returning:  "\<lbrakk>\<Gamma>,\<gamma>,p\<turnstile> rs\<^sub>1 \<Rightarrow>\<^sub>r Undecided; matches \<gamma> m' p\<rbrakk>
     \<Longrightarrow> \<Gamma>,\<gamma>,p\<turnstile> rs\<^sub>1 @ Rule m' Return # rs\<^sub>2 \<Rightarrow>\<^sub>r Undecided"
 proof(induction rs\<^sub>1)
   case Nil
@@ -131,13 +133,13 @@ next
   then show ?case by - (rule iptables_bigstep_r.cases[OF Cons.prems(1)]; simp add: iptables_bigstep_r.intros)
 qed
  
-lemma e: "\<Gamma>,\<gamma>,p\<turnstile> rs \<Rightarrow>\<^sub>z t \<Longrightarrow> s = Undecided \<Longrightarrow> \<Gamma>,\<gamma>,p\<turnstile> rs \<Rightarrow>\<^sub>r t"
+private lemma e: "\<Gamma>,\<gamma>,p\<turnstile> rs \<Rightarrow>\<^sub>z t \<Longrightarrow> s = Undecided \<Longrightarrow> \<Gamma>,\<gamma>,p\<turnstile> rs \<Rightarrow>\<^sub>r t"
   by(induction rule: iptables_bigstep_nz.induct; simp add: iptables_bigstep_r.intros returning)
     
 
 definition "no_call_to c rs \<equiv> (\<forall>r \<in> set rs. case get_action r of Call c' \<Rightarrow> c \<noteq> c' | _ \<Rightarrow> True)"
 definition "all_chains p \<Gamma> rs \<equiv> (p rs \<and> (\<forall>l rs. \<Gamma> l = Some rs \<longrightarrow> p rs))"
-lemma all_chains_no_call_upd: "all_chains (no_call_to c) \<Gamma> rs \<Longrightarrow> (\<Gamma>(c \<mapsto> x)),\<gamma>,p\<turnstile> rs \<Rightarrow>\<^sub>z t \<longleftrightarrow> \<Gamma>,\<gamma>,p\<turnstile> rs \<Rightarrow>\<^sub>z t"
+private lemma all_chains_no_call_upd: "all_chains (no_call_to c) \<Gamma> rs \<Longrightarrow> (\<Gamma>(c \<mapsto> x)),\<gamma>,p\<turnstile> rs \<Rightarrow>\<^sub>z t \<longleftrightarrow> \<Gamma>,\<gamma>,p\<turnstile> rs \<Rightarrow>\<^sub>z t"
 proof (rule iffI, goal_cases)
   case 1
   from 1(2,1) show ?case 
@@ -153,19 +155,19 @@ qed
 lemma updated_call: "\<Gamma>(c \<mapsto> rs),\<gamma>,p\<turnstile> rs \<Rightarrow>\<^sub>z t \<Longrightarrow> matches \<gamma> m p \<Longrightarrow> \<Gamma>(c \<mapsto> rs),\<gamma>,p\<turnstile> [Rule m (Call c)] \<Rightarrow>\<^sub>z t"
   by(cases t; simp add: iptables_bigstep_nz.call_no_result iptables_bigstep_nz.call_result iptables_bigstep_nz.skip)
     
-lemma shows
+private lemma shows
       log_nz:     "\<Gamma>,\<gamma>,p\<turnstile> rs \<Rightarrow>\<^sub>z t \<Longrightarrow> \<Gamma>,\<gamma>,p\<turnstile> Rule m Log # rs \<Rightarrow>\<^sub>z t"
 and empty_nz:   "\<Gamma>,\<gamma>,p\<turnstile> rs \<Rightarrow>\<^sub>z t \<Longrightarrow> \<Gamma>,\<gamma>,p\<turnstile> Rule m Empty # rs \<Rightarrow>\<^sub>z t"
   by (meson iptables_bigstep_nz.log iptables_bigstep_nz.empty iptables_bigstep_nz.nms)+
     
-lemma nz_empty_rs_stateD: assumes "\<Gamma>,\<gamma>,p\<turnstile> [] \<Rightarrow>\<^sub>z t" shows "t = Undecided"
+private lemma nz_empty_rs_stateD: assumes "\<Gamma>,\<gamma>,p\<turnstile> [] \<Rightarrow>\<^sub>z t" shows "t = Undecided"
   using assms by(cases rule: iptables_bigstep_nz.cases)
     
-lemma upd_callD: "\<Gamma>(c \<mapsto> rs),\<gamma>,p\<turnstile> [Rule m (Call c)] \<Rightarrow>\<^sub>z t \<Longrightarrow> matches \<gamma> m p 
+private lemma upd_callD: "\<Gamma>(c \<mapsto> rs),\<gamma>,p\<turnstile> [Rule m (Call c)] \<Rightarrow>\<^sub>z t \<Longrightarrow> matches \<gamma> m p 
   \<Longrightarrow> (\<Gamma>(c \<mapsto> rs),\<gamma>,p\<turnstile> rs \<Rightarrow>\<^sub>z t \<or> (\<exists>rs\<^sub>1 rs\<^sub>2 m'. rs = rs\<^sub>1 @ Rule m' Return # rs\<^sub>2 \<and> matches \<gamma> m' p \<and> \<Gamma>(c \<mapsto> rs),\<gamma>,p\<turnstile> rs\<^sub>1 \<Rightarrow>\<^sub>z Undecided \<and> t = Undecided))"
   by(subst (asm) iptables_bigstep_nz.simps) (auto dest!: nz_empty_rs_stateD)
     
-lemma partial_fun_upd: "(f(x \<mapsto> y)) x = Some y" by(fact fun_upd_same)
+private lemma partial_fun_upd: "(f(x \<mapsto> y)) x = Some y" by(fact fun_upd_same)
  
 lemma f: "\<Gamma>,\<gamma>,p\<turnstile> rs \<Rightarrow>\<^sub>r t \<Longrightarrow> matches \<gamma> m p \<Longrightarrow> all_chains (no_call_to c) \<Gamma> rs \<Longrightarrow> 
   (\<Gamma>(c \<mapsto> rs)),\<gamma>,p\<turnstile> [Rule m (Call c)] \<Rightarrow>\<^sub>z t"
@@ -269,57 +271,82 @@ next
     apply safe (* oh. Didn't expect that. :) *)
   done
 next
-  case (call_no_result m' c' rs rrs t)
-  have acrs: "all_chains (no_call_to c) \<Gamma> rs" using call_no_result(2,8) by(simp add: all_chains_def no_call_to_def)
-  have acrrs: "all_chains (no_call_to c) \<Gamma> rrs" using call_no_result(2,8) by(simp add: all_chains_def no_call_to_def)
+  case (call_no_result c' rs rrs t m')
+  have acrs: "all_chains (no_call_to c) \<Gamma> rs" using call_no_result(1,7) by(simp add: all_chains_def no_call_to_def)
+  have acrrs: "all_chains (no_call_to c) \<Gamma> rrs" using call_no_result(7) by(simp add: all_chains_def no_call_to_def)
   have acrs1: "all_chains (no_call_to c) \<Gamma> rs\<^sub>1" if "rs = rs\<^sub>1 @ rs\<^sub>2" for rs\<^sub>1 rs\<^sub>2
     using acrs that by(simp add: all_chains_def no_call_to_def)
   have acrrs1: "all_chains (no_call_to c) \<Gamma> rs\<^sub>1" if "rrs = rs\<^sub>1 @ rs\<^sub>2" for rs\<^sub>1 rs\<^sub>2
     using acrrs that by(simp add: all_chains_def no_call_to_def)
-  have cc: "c \<noteq> c'" (* okay, this one is a bit nifty\<dots> *) using call_no_result(8) by(simp add: all_chains_def no_call_to_def)
-  have "\<Gamma>(c \<mapsto> rs),\<gamma>,p\<turnstile> [Rule m (Call c)] \<Rightarrow>\<^sub>z Undecided" using call_no_result.IH call_no_result.prems(1) acrs by blast
-  with call_no_result(6)[OF \<open>matches \<gamma> m p\<close> acrrs] show ?case
-    apply -
-    apply(drule upd_callD[OF _ \<open>matches \<gamma> m p\<close>])+
-    apply(elim disjE) (* 4 sg *)
-    apply safe
-    subgoal
-      apply(rule updated_call[OF _ \<open>matches \<gamma> m p\<close>])
-      apply(rule iptables_bigstep_nz.call_no_result[where rs=rs, OF \<open>matches \<gamma> m' p\<close> ])
-      apply(simp add: cc[symmetric] call_no_result(2);fail)
-       apply(simp add: acrs all_chains_no_call_upd;fail)
-      apply(simp add: acrrs all_chains_no_call_upd)
+  have cc: "c \<noteq> c'" (* okay, this one is a bit nifty\<dots> *) using call_no_result(7) by(simp add: all_chains_def no_call_to_def)
+  have *: "\<Gamma>(c \<mapsto> rs),\<gamma>,p\<turnstile> [Rule m (Call c)] \<Rightarrow>\<^sub>z Undecided" using call_no_result.IH call_no_result.prems(1) acrs by blast
+  have **: "\<Gamma>(c \<mapsto> rrs),\<gamma>,p\<turnstile> [Rule m (Call c)] \<Rightarrow>\<^sub>z t" by (simp add: acrrs call_no_result.IH(2) call_no_result.prems(1))
+  show ?case proof(cases \<open>matches \<gamma> m' p\<close>)
+    case True
+    from call_no_result(5)[OF \<open>matches \<gamma> m p\<close> acrrs] * show ?thesis
+      apply -
+      apply(drule upd_callD[OF _ \<open>matches \<gamma> m p\<close>])+
+      apply(elim disjE) (* 4 sg *)
+      apply safe
+      subgoal
+        apply(rule updated_call[OF _ \<open>matches \<gamma> m p\<close>])
+        apply(rule iptables_bigstep_nz.call_no_result[where rs=rs, OF \<open>matches \<gamma> m' p\<close> ])
+        apply(simp add: cc[symmetric] call_no_result(1);fail)
+         apply(simp add: acrs all_chains_no_call_upd;fail)
+        apply(simp add: acrrs all_chains_no_call_upd)
+        done
+      subgoal for rs\<^sub>1 rs\<^sub>2 r
+        apply(rule updated_call[OF _ \<open>matches \<gamma> m p\<close>])
+        apply(rule call_return[OF \<open>matches \<gamma> m' p\<close>])
+           apply(simp add: cc[symmetric] call_no_result(1);fail)
+          apply(simp;fail)
+         apply(simp add: acrs1 all_chains_no_call_upd;fail)
+        apply(simp add: acrrs all_chains_no_call_upd)
+        done
+      subgoal for rs\<^sub>1 rs\<^sub>2 r
+        apply(rule call_return[where rs\<^sub>1="Rule m' (Call c') # rs\<^sub>1", OF \<open>matches \<gamma> m p\<close>])
+           apply(simp;fail)
+          apply(simp;fail)
+        apply(rule iptables_bigstep_nz.call_no_result[OF \<open>matches \<gamma> m' p\<close>])
+           apply(simp add: cc[symmetric] call_no_result(1);fail)
+          apply (meson acrs all_chains_no_call_upd)
+         apply(subst all_chains_no_call_upd; simp add: acrrs1 all_chains_no_call_upd; fail)
+        apply (simp add: iptables_bigstep_nz.skip;fail)
+        done
+      subgoal for rrs\<^sub>1 rs\<^sub>1 rrs\<^sub>2 rs\<^sub>2 rr r
+         apply(rule call_return[where rs\<^sub>1="Rule m' (Call c') # rrs\<^sub>1", OF \<open>matches \<gamma> m p\<close>])
+           apply(simp;fail)
+          apply(simp;fail)
+         apply(rule call_return[OF \<open>matches \<gamma> m' p\<close>])
+            apply(simp add: cc[symmetric] call_no_result(1);fail)
+           apply blast
+          apply (meson acrs1 all_chains_no_call_upd)
+         apply(subst all_chains_no_call_upd; simp add: acrrs1 all_chains_no_call_upd; fail)
+        apply (simp add: iptables_bigstep_nz.skip;fail)
+        done
       done
-    subgoal for rs\<^sub>1 rs\<^sub>2 r
-      apply(rule updated_call[OF _ \<open>matches \<gamma> m p\<close>])
-      apply(rule call_return[OF \<open>matches \<gamma> m' p\<close>])
-         apply(simp add: cc[symmetric] call_no_result(2);fail)
-        apply(simp;fail)
-       apply(simp add: acrs1 all_chains_no_call_upd;fail)
-      apply(simp add: acrrs all_chains_no_call_upd)
+  next
+    case False
+    from iptables_bigstep_nz.nms[OF False] ** show ?thesis 
+      apply -
+      apply(drule upd_callD[OF _ \<open>matches \<gamma> m p\<close>])+
+      apply(elim disjE)
+      subgoal
+        apply(rule updated_call[OF _ \<open>matches \<gamma> m p\<close>])
+        apply(rule iptables_bigstep_nz.nms[OF False])
+        apply(simp add: acrrs all_chains_no_call_upd)
+        done
+      apply safe
+      subgoal for rs\<^sub>1 rs\<^sub>2 r
+        apply(rule call_return[where rs\<^sub>1="Rule m' (Call c') # rs\<^sub>1", OF \<open>matches \<gamma> m p\<close>])
+           apply(simp;fail)
+          apply(simp;fail)
+         apply(rule iptables_bigstep_nz.nms[OF False])
+         apply(subst all_chains_no_call_upd; simp add: acrrs1 all_chains_no_call_upd; fail)
+        apply(simp add: iptables_bigstep_nz.skip;fail)
+        done
       done
-    subgoal for rs\<^sub>1 rs\<^sub>2 r
-      apply(rule call_return[where rs\<^sub>1="Rule m' (Call c') # rs\<^sub>1", OF \<open>matches \<gamma> m p\<close>])
-         apply(simp;fail)
-        apply(simp;fail)
-      apply(rule iptables_bigstep_nz.call_no_result[OF \<open>matches \<gamma> m' p\<close>])
-         apply(simp add: cc[symmetric] call_no_result(2);fail)
-        apply (meson acrs all_chains_no_call_upd)
-       apply(subst all_chains_no_call_upd; simp add: acrrs1 all_chains_no_call_upd; fail)
-      apply (simp add: iptables_bigstep_nz.skip;fail)
-      done
-    subgoal for rrs\<^sub>1 rs\<^sub>1 rrs\<^sub>2 rs\<^sub>2 rr r
-       apply(rule call_return[where rs\<^sub>1="Rule m' (Call c') # rrs\<^sub>1", OF \<open>matches \<gamma> m p\<close>])
-         apply(simp;fail)
-        apply(simp;fail)
-       apply(rule call_return[OF \<open>matches \<gamma> m' p\<close>])
-          apply(simp add: cc[symmetric] call_no_result(2);fail)
-         apply blast
-        apply (meson acrs1 all_chains_no_call_upd)
-       apply(subst all_chains_no_call_upd; simp add: acrrs1 all_chains_no_call_upd; fail)
-      apply (simp add: iptables_bigstep_nz.skip;fail)
-      done
-    done
+  qed
 qed
   
 lemma r_skip_inv: "\<Gamma>,\<gamma>,p\<turnstile> [] \<Rightarrow>\<^sub>r t \<Longrightarrow> t = Undecided"
@@ -335,15 +362,27 @@ lemma r_call_eq: "\<Gamma> c = Some rs \<Longrightarrow> matches \<gamma> m p \<
   done
   subgoal
     apply(cases t)
-     apply(erule (1) iptables_bigstep_r.call_no_result)
+     apply(erule iptables_bigstep_r.call_no_result)
       apply(simp;fail)
      apply(simp add: iptables_bigstep_r.skip;fail)
       apply(simp)
     apply(erule (2) iptables_bigstep_r.call_result)
   done
-by -
+  by -
+
+(* we can make the same formulation for the original semantics if we tread a bit more carefully *)
+lemma call_eq: "\<Gamma> c = Some rs \<Longrightarrow> matches \<gamma> m p \<Longrightarrow> \<forall>r \<in> set rs. get_action r \<noteq> Return  \<Longrightarrow> \<Gamma>,\<gamma>,p\<turnstile> \<langle>[Rule m (Call c)],s\<rangle> \<Rightarrow> t \<longleftrightarrow> \<Gamma>,\<gamma>,p\<turnstile> \<langle>rs,s\<rangle> \<Rightarrow> t"
+  apply(rule iffI)
+  subgoal
+    apply(subst (asm) iptables_bigstep.simps)
+    apply (auto)
+     apply (simp add: decision)
+    apply(erule rules_singleton_rev_E; simp; metis callD in_set_conv_decomp rule.sel(2) skipD)
+  done
+  by (metis decision iptables_bigstep.call_result iptables_bigstep_deterministic state.exhaust)
   
-theorem r_eq_orig: "\<lbrakk>all_chains (no_call_to c) \<Gamma> rs; \<Gamma> c = Some rs\<rbrakk> \<Longrightarrow> \<Gamma>,\<gamma>,p\<turnstile> rs \<Rightarrow>\<^sub>r t \<longleftrightarrow> \<Gamma>,\<gamma>,p\<turnstile> \<langle>[Rule MatchAny (Call c)], Undecided\<rangle> \<Rightarrow> t"
+theorem r_eq_orig: "\<lbrakk>all_chains (no_call_to c) \<Gamma> rs; \<Gamma> c = Some rs\<rbrakk> \<Longrightarrow>
+   \<Gamma>,\<gamma>,p\<turnstile> rs \<Rightarrow>\<^sub>r t \<longleftrightarrow> \<Gamma>,\<gamma>,p\<turnstile> \<langle>[Rule MatchAny (Call c)], Undecided\<rangle> \<Rightarrow> t"
   apply(rule iffI)
   subgoal
     apply(drule f[where m=MatchAny, THEN c, THEN a])
@@ -358,10 +397,220 @@ theorem r_eq_orig: "\<lbrakk>all_chains (no_call_to c) \<Gamma> rs; \<Gamma> c =
     apply(erule b[THEN d, THEN e, OF _ refl refl refl])
     done
   done
+    
+lemma r_no_call: "\<Gamma>,\<gamma>,p\<turnstile> Rule MatchAny (Call c)#rs \<Rightarrow>\<^sub>r t \<Longrightarrow> \<Gamma> c = None \<Longrightarrow> False"
+  by(subst (asm) iptables_bigstep_r.simps) simp
+    
+lemma no_call: "\<Gamma>,\<gamma>,p\<turnstile> \<langle>rs, s\<rangle> \<Rightarrow> t \<Longrightarrow> rs = [Rule MatchAny (Call c)] \<Longrightarrow> s = Undecided \<Longrightarrow> \<Gamma> c = None \<Longrightarrow> False"
+  by (meson b d e r_no_call)
+  (*by(induction rule: iptables_bigstep.induct; clarsimp) (metis list_app_singletonE skipD)*)
 
-corollary r_eq_orig': "\<lbrakk>all_chains (no_call_to c) \<Gamma> rs; \<Gamma> c = Some rs\<rbrakk> \<Longrightarrow> 
-  \<Gamma>,\<gamma>,p\<turnstile> [Rule MatchAny (Call c)] \<Rightarrow>\<^sub>r t \<longleftrightarrow> \<Gamma>,\<gamma>,p\<turnstile> \<langle>[Rule MatchAny (Call c)], Undecided\<rangle> \<Rightarrow> t"
+private corollary r_eq_orig': assumes "\<forall>rs \<in> ran \<Gamma>. no_call_to c rs"
+  shows "\<Gamma>,\<gamma>,p\<turnstile> [Rule MatchAny (Call c)] \<Rightarrow>\<^sub>r t \<longleftrightarrow> \<Gamma>,\<gamma>,p\<turnstile> \<langle>[Rule MatchAny (Call c)], Undecided\<rangle> \<Rightarrow> t"
 (* if you really like symmetry *)
-  by(simp add: r_call_eq r_eq_orig)
+proof -
+  show ?thesis proof (cases "\<Gamma> c")
+    fix rs
+    assume "\<Gamma> c = Some rs"
+    moreover hence "all_chains (no_call_to c) \<Gamma> rs" using assms by (simp add: all_chains_def ranI)
+    ultimately show ?thesis by(simp add: r_call_eq r_eq_orig)
+  next
+    assume "\<Gamma> c = None" thus ?thesis using r_no_call no_call by metis
+  qed
+qed
+  
+(* btw, we can still formulate a seq rules, but we have to tread a bit more carefully *)
+lemma r_tail: assumes "\<Gamma>,\<gamma>,p\<turnstile> rs1 \<Rightarrow>\<^sub>r Decision X" shows "\<Gamma>,\<gamma>,p\<turnstile> rs1 @ rs2 \<Rightarrow>\<^sub>r Decision X"
+proof -
+  have "\<Gamma>,\<gamma>,p\<turnstile> rs1 \<Rightarrow>\<^sub>r t \<Longrightarrow> t = Decision X \<Longrightarrow> \<Gamma>,\<gamma>,p\<turnstile> rs1 @ rs2 \<Rightarrow>\<^sub>r Decision X" for t
+    by(induction rule: iptables_bigstep_r.induct; simp add: iptables_bigstep_r.intros)
+  thus ?thesis using assms by blast
+qed
+lemma r_seq: "\<Gamma>,\<gamma>,p\<turnstile> rs1 \<Rightarrow>\<^sub>r Undecided \<Longrightarrow> \<forall>r \<in> set rs1. \<not>(get_action r = Return \<and> matches \<gamma> (get_match r) p)
+   \<Longrightarrow> \<Gamma>,\<gamma>,p\<turnstile> rs2 \<Rightarrow>\<^sub>r t \<Longrightarrow> \<Gamma>,\<gamma>,p\<turnstile> rs1 @ rs2 \<Rightarrow>\<^sub>r t"
+proof(induction rs1)
+  case Nil
+  then show ?case by simp
+next
+  case (Cons r rs1)
+  have p2: "\<forall>r\<in>set rs1. \<not> (get_action r = Return \<and> matches \<gamma> (get_match r) p)" 
+           "\<not>(get_action r = Return \<and> matches \<gamma> (get_match r) p)"
+    by (simp_all add: Cons.prems(2))
+  from Cons.prems(1) p2(2) Cons.IH[OF _ p2(1) Cons.prems(3)] show ?case 
+    by(cases rule: iptables_bigstep_r.cases; simp add: iptables_bigstep_r.intros)
+qed
+
+lemma r_appendD: "\<Gamma>,\<gamma>,p\<turnstile> rs1 @ rs2 \<Rightarrow>\<^sub>r t \<Longrightarrow> \<exists>s. \<Gamma>,\<gamma>,p\<turnstile> rs1 \<Rightarrow>\<^sub>r s"
+  proof(induction rs1)
+    case (Cons r rs1)
+    from Cons.prems Cons.IH show ?case by(cases rule: iptables_bigstep_r.cases) (auto intro: iptables_bigstep_r.intros)
+  qed (meson iptables_bigstep_r.skip)
+
+corollary iptables_bigstep_r_eq: assumes "\<forall>rs \<in> ran \<Gamma>. no_call_to c rs" "A = Accept \<or> A = Drop"
+  shows "\<Gamma>,\<gamma>,p\<turnstile> [Rule MatchAny (Call c), Rule MatchAny A] \<Rightarrow>\<^sub>r t \<longleftrightarrow> \<Gamma>,\<gamma>,p\<turnstile> \<langle>[Rule MatchAny (Call c), Rule MatchAny A], Undecided\<rangle> \<Rightarrow> t"
+(* if you really like the way we do our analyses *)
+proof -
+  show ?thesis proof (cases "\<Gamma> c")
+    fix rs
+    assume "\<Gamma> c = Some rs"
+    moreover hence "all_chains (no_call_to c) \<Gamma> rs" using assms by (simp add: all_chains_def ranI)
+    show ?thesis
+      (* if this proof breaks, don't fix it. say 'meh' and re-prove this as a corollary of r_eq_orig''' with a stronger assumption *)
+      apply(rule iffI[rotated])
+       apply(erule seqE_cons)
+       apply(subst (asm) r_eq_orig'[symmetric])
+        apply (simp add: assms(1);fail)
+       apply (meson assms(1) b d e r_eq_orig' seq'_cons) (* holy shi\<dots> *)
+      apply(frule r_appendD[of _ _ _ "[Rule MatchAny (Call c)]" "[Rule MatchAny A]", simplified])
+      apply(subst (asm) r_eq_orig')
+        apply (simp add: assms(1);fail)
+        apply(clarsimp)
+      apply(subst (asm) r_eq_orig'[symmetric])
+       apply (simp add: assms(1);fail)
+      apply(subst (asm)(2) iptables_bigstep_r.simps)
+      apply(subst (asm)(1) iptables_bigstep_r.simps)
+      apply auto
+         apply (metis append_Cons append_Nil assms(1) decision matches.simps(4) r_call_eq r_eq_orig' seq)
+        apply (metis \<open>all_chains (no_call_to c) \<Gamma> rs\<close> calculation iptables_bigstep_deterministic option.inject r_eq_orig state.distinct(1))
+      subgoal using \<open>all_chains (no_call_to c) \<Gamma> rs\<close> calculation iptables_bigstep_deterministic r_eq_orig by fastforce
+      apply(subst (asm) r_eq_orig[rotated])
+        apply(assumption)
+      subgoal using \<open>all_chains (no_call_to c) \<Gamma> rs\<close> calculation by simp
+      apply(erule seq'_cons)
+      apply(subst (asm)(1) iptables_bigstep_r.simps)  
+      apply(insert assms(2); auto simp add: iptables_bigstep.intros)
+      done        
+  next
+    assume "\<Gamma> c = None" thus ?thesis using r_no_call no_call by (metis seqE_cons)
+  qed
+qed
+
+(* now, you don't like that no_call_to assumption? this one's for you: *)
+lemma ex_no_call: "finite S \<Longrightarrow> \<exists>c. \<forall>(rs :: 'a rule list) \<in> S. no_call_to c rs"
+(* If you want, you can put in \<open>ran \<Gamma>\<close> for S. *)
+proof -
+  assume fS: \<open>finite S\<close>
+  def called_c \<equiv> "\<lambda>rs :: 'a rule list. {c. \<exists>m. Rule m (Call c) \<in> set rs}"
+  def called_c' \<equiv> "\<lambda>rs :: 'a rule list. set [c. r \<leftarrow> rs, c \<leftarrow> (case get_action r of Call c \<Rightarrow> [c] | _ \<Rightarrow> [])]"
+  have cc: "called_c' rs = called_c rs" for rs
+    unfolding called_c'_def called_c_def
+    by(induction rs; simp add: Un_def) (auto; metis rule.collapse)      
+  have f: "finite (called_c rs)" for rs unfolding cc[symmetric] called_c'_def by blast
+  have ncc: "no_call_to c rs \<longleftrightarrow> c \<notin> called_c rs" for c rs 
+    by(induction rs; auto simp add: no_call_to_def called_c_def split: action.splits) (metis rule.collapse)
+  have isu: "infinite (UNIV :: string set)" by (simp add: infinite_UNIV_listI)
+  have ff: "finite (\<Union>rs \<in> S. called_c rs)" using f fS by simp
+  then obtain c where ne: "c \<notin> (\<Union>rs \<in> S. called_c rs)"
+    by (blast dest: ex_new_if_finite[OF isu])
+  thus ?thesis by(intro exI[where x=c]) (simp add: ncc)
+  (* stupid way of proving something, once again\<dots> *)
+qed
+
+private lemma ex_no_call': "finite (dom \<Gamma>) \<Longrightarrow> \<exists>c. \<Gamma> c = None \<and> (\<forall>(rs :: 'a rule list) \<in> (ran \<Gamma>). no_call_to c rs)"
+(* I want a corollary, and I need something a tad stronger\<dots> *)
+proof -
+  have *: "finite S \<Longrightarrow> (dom M) = S \<Longrightarrow> \<exists>m. M = map_of m" for M S
+  proof(induction arbitrary: M rule: finite.induct)
+    case emptyI
+    then show ?case by(intro exI[where x=Nil]) simp
+  next
+    case (insertI A a)
+    show ?case proof(cases "a \<in> A") (* stupid induction rule *)
+      case True
+      then show ?thesis using insertI by (simp add: insert_absorb)
+    next
+      case False
+      hence "dom (M(a := None)) = A" using insertI.prems by simp
+      from insertI.IH[OF this] obtain m where "M(a := None) = map_of m" ..
+      then show ?thesis 
+        by(intro exI[where x="(a, the (M a)) # m"]) (simp; metis domIff fun_upd_apply insertCI insertI.prems option.collapse)
+    qed
+  qed (* hm, thought that would give me what I want\<dots> *)
+  have ran_alt: "ran f = (the o f) ` dom f" for f by(auto simp add: ran_def dom_def image_def)
+  assume fD: \<open>finite (dom \<Gamma>)\<close>
+  hence fS: \<open>finite (ran \<Gamma>)\<close> by(simp add: ran_alt)
+  def called_c \<equiv> "\<lambda>rs :: 'a rule list. {c. \<exists>m. Rule m (Call c) \<in> set rs}"
+  def called_c' \<equiv> "\<lambda>rs :: 'a rule list. set [c. r \<leftarrow> rs, c \<leftarrow> (case get_action r of Call c \<Rightarrow> [c] | _ \<Rightarrow> [])]"
+  have cc: "called_c' rs = called_c rs" for rs
+    unfolding called_c'_def called_c_def
+    by(induction rs; simp add: Un_def) (auto; metis rule.collapse)      
+  have f: "finite (called_c rs)" for rs unfolding cc[symmetric] called_c'_def by blast
+  have ncc: "no_call_to c rs \<longleftrightarrow> c \<notin> called_c rs" for c rs 
+    by(induction rs; auto simp add: no_call_to_def called_c_def split: action.splits) (metis rule.collapse) 
+  have isu: "infinite (UNIV :: string set)" by (simp add: infinite_UNIV_listI)
+  have ff: "finite (\<Union>rs \<in> ran \<Gamma>. called_c rs)" using f fS by simp
+  hence fff: "finite (dom \<Gamma> \<union> (\<Union>rs \<in> ran \<Gamma>. called_c rs))" using fD by simp
+  then obtain c where ne: "c \<notin> (dom \<Gamma> \<union> (\<Union>rs \<in> ran \<Gamma>. called_c rs))" thm ex_new_if_finite
+    by (metis UNIV_I isu set_eqI)
+  thus ?thesis by(fastforce simp add: ncc)
+qed
+  
+lemma all_chains_no_call_upd_r: "all_chains (no_call_to c) \<Gamma> rs \<Longrightarrow> (\<Gamma>(c \<mapsto> x)),\<gamma>,p\<turnstile> rs \<Rightarrow>\<^sub>r t \<longleftrightarrow> \<Gamma>,\<gamma>,p\<turnstile> rs \<Rightarrow>\<^sub>r t"
+proof (rule iffI, goal_cases)
+  case 1
+  from 1(2,1) show ?case 
+    by(induction rule: iptables_bigstep_r.induct; 
+      (simp add: iptables_bigstep_r.intros no_call_to_def all_chains_def split: if_splits;fail)?)
+next
+  case 2
+  from 2(2,1) show ?case 
+    by(induction rule: iptables_bigstep_r.induct; 
+      (simp add: iptables_bigstep_r.intros no_call_to_def all_chains_def split:  action.splits;fail)?)
+qed
+
+(* in a sense, this is code duplication with Ruleset_Update, but it's different enough that I can't use it. *)
+lemma all_chains_no_call_upd_orig: "all_chains (no_call_to c) \<Gamma> rs \<Longrightarrow> (\<Gamma>(c \<mapsto> x)),\<gamma>,p\<turnstile> \<langle>rs,s\<rangle> \<Rightarrow> t \<longleftrightarrow> \<Gamma>,\<gamma>,p\<turnstile> \<langle>rs,s\<rangle> \<Rightarrow> t"
+proof (rule iffI, goal_cases)
+  case 1
+  from 1(2,1) show ?case 
+    by(induction rs s t rule: iptables_bigstep.induct; 
+      (simp add: iptables_bigstep.intros no_call_to_def all_chains_def split: if_splits;fail)?)
+next
+  case 2
+  from 2(2,1) show ?case 
+    by(induction rule: iptables_bigstep.induct; 
+      (simp add: iptables_bigstep.intros no_call_to_def all_chains_def split:  action.splits;fail)?)
+qed
+  
+  
+corollary r_eq_orig''': assumes "finite (ran \<Gamma>)" and "\<forall>r \<in> set rs. get_action r \<noteq> Return"
+  shows "\<Gamma>,\<gamma>,p\<turnstile> rs \<Rightarrow>\<^sub>r t \<longleftrightarrow> \<Gamma>,\<gamma>,p\<turnstile> \<langle>rs, Undecided\<rangle> \<Rightarrow> t"
+proof -
+  from assms have "finite ({rs} \<union> (ran \<Gamma>))" by simp
+  from ex_no_call[OF this] obtain c where c: "(\<forall>rs\<in>ran \<Gamma>. no_call_to c rs)" "no_call_to c rs" by blast
+  hence acnc: "all_chains (no_call_to c) \<Gamma> rs" unfolding all_chains_def by (simp add: ranI)
+  have ranaway: "\<forall>rs\<in>ran (\<Gamma>(c \<mapsto> rs)). no_call_to c rs"
+  proof -
+    { (* hammer *)
+      fix rsa :: "'a rule list"
+      assume a1: "rsa \<in> ran (\<Gamma>(c \<mapsto> rs))"
+      have "\<And>R. rs \<in> R \<union> Collect (no_call_to c)"
+        using c(2) by force
+      then have "rsa \<in> ran (\<Gamma>(c := None)) \<union> Collect (no_call_to c)"
+        using a1 by (metis (no_types) Un_iff Un_insert_left fun_upd_same fun_upd_upd insert_absorb ran_map_upd)
+      then have "no_call_to c rsa"
+        by (metis (no_types) Un_iff c(1) mem_Collect_eq ranI ran_restrictD restrict_complement_singleton_eq)
+    }
+    thus ?thesis by simp
+  qed
+  have "\<Gamma>(c \<mapsto> rs),\<gamma>,p\<turnstile> rs \<Rightarrow>\<^sub>r t \<longleftrightarrow> \<Gamma>(c \<mapsto> rs),\<gamma>,p\<turnstile> \<langle>rs, Undecided\<rangle> \<Rightarrow> t"
+    apply(subst r_call_eq[where c=c and m=MatchAny,symmetric])
+      apply(simp;fail)
+     apply(simp;fail)
+    apply(subst call_eq[where c=c and m=MatchAny,symmetric])
+      apply(simp;fail)
+      apply(simp;fail)
+     apply(simp add: assms;fail)
+    apply(rule r_eq_orig')
+    apply(fact ranaway)
+    done
+  thus ?thesis 
+    apply -
+    apply(subst (asm) all_chains_no_call_upd_r[where x=rs, OF acnc])
+    apply(subst (asm) all_chains_no_call_upd_orig[where x=rs, OF acnc])
+    .
+qed
+
+end
 
 end
